test/test_either_unit_unit.v
@@ -1,12 +1,12 @@
 (*! sv:reject cpp:reject *)
-From stdpp Require Import bitvector.definitions.
+From Stdlib Require Import Bits.
 From Stdlib Require Import BinInt String List.
 Require Import quartz.lang.Syntax. Import type.
 Import (notations) type expr eexpr.
 Local Open Scope string_scope.
 
 Definition test_either_unit_unit_inner {var} := @fn.Fn var type.Unit (Either Unit Unit) (fun _ =>
-  eexpr.Ret (expr.Unop unop.Left (expr.Const (t:=Unit) (bv_0 _)))
+  eexpr.Ret (expr.Unop unop.Left (expr.Const (t:=Unit) Zmod.zero))
 ).
 
 Definition test_either_unit_unit {var fn} := fns.package_global_fns'' var fn (@test_either_unit_unit_inner).
